git/JLimperg/aesop/Aesop/Index.lean
@@ -1,0 +1,138 @@
+/-
+Copyright (c) 2021 Jannis Limperg. All rights reserved.
+Released under Apache 2.0 license as described in the file LICENSE.
+Authors: Jannis Limperg
+-/
+
+import Aesop.Index.Basic
+
+open Lean
+open Lean.Meta
+open Std (RBMap mkRBMap PHashSet)
+
+namespace Aesop
+
+structure Index (α : Type) [BEq α] [Hashable α] where
+  byTarget : DiscrTree α
+  byHyp : DiscrTree α
+  unindexed : PHashSet α
+  deriving Inhabited
+
+namespace Index
+
+variable [BEq α] [Hashable α]
+
+open MessageData in
+instance [ToMessageData α] : ToMessageData (Index α) where
+  toMessageData ri := node #[
+    "indexed by target:" ++ node (ri.byTarget.values.map toMessageData),
+    "indexed by hypotheses:" ++ node (ri.byHyp.values.map toMessageData),
+    "unindexed:" ++ node (ri.unindexed.toArray.map toMessageData)
+  ]
+
+instance : EmptyCollection (Index α) where
+  emptyCollection := {
+    byTarget := {}
+    byHyp := {}
+    unindexed := {}
+  }
+
+def merge (ri₁ ri₂ : Index α) : Index α where
+  byTarget := ri₁.byTarget.merge ri₂.byTarget
+  byHyp := ri₁.byHyp.merge ri₂.byHyp
+  unindexed := ri₁.unindexed.merge ri₂.unindexed
+
+@[specialize]
+partial def add (r : α) (imode : IndexingMode) (ri : Index α) :
+    Index α :=
+  match imode with
+  | IndexingMode.unindexed =>
+    { ri with unindexed := ri.unindexed.insert r }
+  | IndexingMode.target keys =>
+    { ri with byTarget := ri.byTarget.insertCore keys r }
+  | IndexingMode.hyps keys =>
+    { ri with byHyp := ri.byHyp.insertCore keys r }
+  | IndexingMode.or imodes =>
+    imodes.foldl (init := ri) λ ri imode =>
+      ri.add r imode
+
+def foldM [Monad m] (ri : Index α) (f : σ → α → m σ) (init : σ) : m σ :=
+  match ri with
+  | { byHyp, byTarget, unindexed} => do
+    let mut s := init
+    s ← byHyp.foldValuesM (init := s) f
+    s ← byTarget.foldValuesM (init := s) f
+    unindexed.foldM (init := s) f
+
+@[inline]
+def fold (ri : Index α) (f : σ → α → σ) (init : σ) : σ :=
+  Id.run $ ri.foldM (init := init) f
+
+def size : Index α → Nat
+  | { byHyp, byTarget, unindexed } =>
+    byHyp.size + byTarget.size + unindexed.size
+
+-- May return duplicate `IndexMatchLocation`s.
+@[inline]
+private def applicableByTargetRules (ri : Index α) (goal : MVarId)
+    (include? : α → Bool) : MetaM (Array (α × Array IndexMatchLocation)) :=
+  withMVarContext goal do
+    let rules ←
+      ri.byTarget.getUnifyWithTransparency (← getMVarType goal)
+        indexingTransparency
+    let mut rs := Array.mkEmpty rules.size
+      -- Assumption: include? is true for most rules.
+    for r in rules do
+      if include? r then
+        rs := rs.push (r, #[.target])
+    return rs
+
+-- May return duplicate `IndexMatchLocation`s.
+@[inline]
+private def applicableByHypRules (ri : Index α) (goal : MVarId)
+    (include? : α → Bool) : MetaM (Array (α × Array IndexMatchLocation)) :=
+  withMVarContext goal do
+    let mut rs := #[]
+    for localDecl in ← getLCtx do
+      if localDecl.isAuxDecl then continue
+      let rules ←
+        ri.byHyp.getUnifyWithTransparency localDecl.type indexingTransparency
+      for r in rules do
+        if include? r then
+          rs := rs.push (r, #[.hyp localDecl])
+    return rs
+
+-- May return duplicate `IndexMatchLocation`s.
+@[inline]
+private def applicableUnindexedRules (ri : Index α) (include? : α → Bool) :
+    Array (α × Array IndexMatchLocation) :=
+  -- Assumption: include? is true for most rules.
+  ri.unindexed.fold (init := Array.mkEmpty ri.unindexed.size) λ acc r =>
+    if include? r then
+      acc.push (r, #[.none])
+    else
+      acc
+
+-- Returns the rules in the order given by the `Ord α` instance.
+@[specialize]
+def applicableRules [ord : Ord α] (ri : Index α) (goal : MVarId)
+    (include? : α → Bool) : MetaM (Array (IndexMatchResult α)) := do
+  instantiateMVarsInGoal goal
+  let mut result := mkRBMap α (Array IndexMatchLocation) compare
+  result := insertIndexMatchResults result
+    (← applicableByTargetRules ri goal include?)
+  result := insertIndexMatchResults result
+    (← applicableByHypRules ri goal include?)
+  result := insertIndexMatchResults result
+    (applicableUnindexedRules ri include?)
+  return result.fold (init := Array.mkEmpty result.size) λ rs rule locs =>
+    rs.push { rule := rule, locations := .ofArray locs }
+  where
+    @[inline]
+    insertIndexMatchResults (m : RBMap α (Array IndexMatchLocation) compare)
+        (rs : Array (α × Array IndexMatchLocation)) :
+        RBMap α (Array IndexMatchLocation) compare :=
+      rs.foldl (init := m) λ m (rule, locs) =>
+        m.insertWith rule locs (· ++ locs)
+
+end Aesop.Index
