git/JLimperg/aesop/Aesop/Index/Basic.lean
@@ -1,0 +1,108 @@
+/-
+Copyright (c) 2021 Jannis Limperg. All rights reserved.
+Released under Apache 2.0 license as described in the file LICENSE.
+Authors: Jannis Limperg
+-/
+
+import Aesop.Util
+
+open Lean
+open Lean.Meta
+open Std (RBMap)
+
+namespace Aesop
+
+-- We use default transparency when indexing values. This means that when a rule
+-- is added to a `DiscrTree` index, the index pattern is normalised with default
+-- transparency, and when a part of the goal (target or hyp) is matched against
+-- the index, it is also normalised with default transparency.
+--
+-- In Lean core, `DiscrTree`s are only used with `reducible` transparency. We
+-- want more computation to avoid weakening rules: if we work up to `reducible`
+-- computation, `apply` is weaker when indexed than when not indexed (and the
+-- same applies to many other rules). The tradeoff is obviously performance and
+-- there may be other unforeseen side effects.
+def indexingTransparency := TransparencyMode.default
+
+inductive IndexingMode : Type
+  | unindexed
+  | target (keys : Array DiscrTree.Key)
+  | hyps (keys : Array DiscrTree.Key)
+  | or (imodes : Array IndexingMode)
+  deriving Inhabited
+
+namespace IndexingMode
+
+protected partial def format : IndexingMode → Format
+  | unindexed => "unindexed"
+  | target keys => f!"target {keys}"
+  | hyps keys => f!"hyps {keys}"
+  | or imodes => f!"or {imodes.map IndexingMode.format}"
+
+instance : ToFormat IndexingMode :=
+  ⟨IndexingMode.format⟩
+
+def targetMatchingConclusion (type : Expr) : MetaM IndexingMode := do
+  let path ← DiscrTree.getConclusionKeys type indexingTransparency
+  return target path
+
+def hypsMatchingConst (decl : Name) : MetaM IndexingMode := do
+  let path ← DiscrTree.getConstKeys decl
+  return hyps path
+
+end IndexingMode
+
+
+inductive IndexMatchLocation
+  | target
+  | none
+  | hyp (ldecl : LocalDecl)
+  deriving Inhabited
+
+namespace IndexMatchLocation
+
+instance : ToMessageData IndexMatchLocation where
+  toMessageData
+    | target => "target"
+    | none => "none"
+    | hyp ldecl => m!"hyp {ldecl.userName}"
+
+instance : BEq IndexMatchLocation where
+  beq
+    | target, target => true
+    | none, none => true
+    | hyp ldecl₁, hyp ldecl₂ => ldecl₁.fvarId == ldecl₂.fvarId
+    | _, _ => false
+
+instance : Ord IndexMatchLocation where
+  compare
+    | target, target => .eq
+    | target, none => .lt
+    | target, hyp .. => .lt
+    | none, target => .gt
+    | none, none => .eq
+    | none, hyp .. => .lt
+    | hyp .., target => .gt
+    | hyp .., none => .gt
+    | hyp ldecl₁, hyp ldecl₂ => ldecl₁.fvarId.name.quickCmp ldecl₂.fvarId.name
+
+end IndexMatchLocation
+
+
+structure IndexMatchResult (α : Type) where
+  rule : α
+  locations : UnorderedArraySet IndexMatchLocation
+  deriving Inhabited
+
+namespace IndexMatchResult
+
+instance [Ord α] : Ord (IndexMatchResult α) where
+  compare r s := compare r.rule s.rule
+
+instance [Ord α] : LT (IndexMatchResult α) :=
+  ltOfOrd
+
+instance [ToMessageData α] : ToMessageData (IndexMatchResult α) where
+  toMessageData r := toMessageData r.rule
+
+end Aesop.IndexMatchResult
